Lean4Lean/Verify/TypeChecker/IsDefEq.lean
@@ -281,15 +281,20 @@ theorem isDefEqApp.WF {c : VContext} {s : VState}
   simp [Expr.getAppArgs_toList, Expr.mkAppList_getAppArgsList] at h2
   exact h2 hb _ he₁ _ he₂
 
+theorem getSortLevel.WF
+    (he : c.TrExprS e e') : (getSortLevel e).WF c s fun l _ =>
+      ∃ u', VLevel.ofLevel c.lparams l = some u' ∧ c.HasType e' (.sort u') := by
+  refine (inferType.WF he).bind fun ty _ le ⟨ty', _, _, h1, h2⟩ => ?_
+  refine (ensureSortCore.WF h1).bind fun ty _ le h => ?_
+  obtain ⟨⟨u, rfl⟩, ⟨ty₂, h3, h4⟩, _⟩ := h
+  let .sort hu := h3
+  exact .pure ⟨_, hu, h2.defeqU_r c.Ewf c.Δwf h4.symm⟩
+
 theorem isProp.WF
     (he : c.TrExprS e e') : (isProp e).WF c s fun b _ => b → c.HasType e' (.sort .zero) := by
-  unfold isProp
-  refine (inferType.WF he).bind fun ty _ le ⟨ty', _, _, h1, h2⟩ => ?_
-  refine .stateWF fun wf => ?_
-  refine (whnf.WF h1).bind fun ty _ le ⟨_, ty₂, h3, h4⟩ => .pure ?_
-  simp [Expr.prop, Expr.eqv_sort]; rintro rfl
-  let .sort h3 := h3; cases h3
-  exact h2.defeqU_r c.Ewf c.Δwf h4.symm
+  refine (getSortLevel.WF he).bind fun l _ le ⟨u', hu, h⟩ => .pure fun H => ?_
+  exact h.defeqU_r c.Ewf c.Δwf
+    ⟨_, .sortDF (.of_ofLevel hu) trivial (ofLevel_isAlwaysZero hu H)⟩
 
 theorem isDefEqProofIrrel.WF {c : VContext} {s : VState}
     (he₁ : c.TrExprS e₁ e₁') (he₂ : c.TrExprS e₂ e₂') :
